Current.thy
@@ -24,9 +24,11 @@ fun isEmpty :: "'a current \<Rightarrow> bool" where
   "isEmpty (Current [] _ old _) = Stack.isEmpty old"
 | "isEmpty _ = False"
 
+(*
+   TODO:
+   Maybe it is needed to find out what the max differences between size old and remained are
+ *)
 fun invariant :: "'a current \<Rightarrow> bool" where
-  "invariant (Current extra added old remained) \<longleftrightarrow> 
-     length extra = added
-   \<and> Stack.size old = remained"
+  "invariant (Current extra added old remained) \<longleftrightarrow> length extra = added"
 
 end
