Idle.thy
@@ -14,7 +14,10 @@ fun pop :: "'a idle \<Rightarrow> ('a * 'a idle)" where
   "pop (Idle stack stackSize) = (Stack.first stack, Idle (Stack.pop stack) (stackSize - 1))"
 
 fun size :: "'a idle \<Rightarrow> nat" where
-  "size (Idle _ stackSize) = stackSize"
+  "size (Idle stack _) = Stack.size stack"
+
+fun isEmpty :: "'a idle \<Rightarrow> bool" where
+  "isEmpty (Idle stack _) \<longleftrightarrow> Stack.isEmpty stack"
 
 fun invariant :: "'a idle \<Rightarrow> bool" where
   "invariant (Idle stack stackSize) \<longleftrightarrow> Stack.size stack = stackSize"
