Big_Proof.thy
@@ -10,17 +10,22 @@ lemma tick: "toList (tick state) = toList state"
   apply(induction state)
   by(auto simp: helper tick)
 
-lemma helper_1: "tick (Reverse current big auxB count) = Reverse current' big' auxB' count' 
-            \<Longrightarrow> Current.invariant current 
-            \<Longrightarrow> Current.invariant current'"
-  apply(induction "(Reverse current big auxB count)" arbitrary: big auxB count big' auxB' count' rule: tick.induct)
-  by auto
-
 lemma invariant_tick: "invariant state \<Longrightarrow> invariant (tick state)"
-  apply(induction state rule: tick.induct)
-    apply(auto simp: rev_take invariant_tick split: current.splits)
-  (* TODO: *)
-  by (smt (z3) Nat.diff_diff_right Stack_Proof.pop Suc_le_D add_Suc_right append_Nil2 diff_diff_cancel diff_less empty first length_drop length_rev nat_less_le size_listLength take_Nil take_Suc zero_less_Suc)
+proof(induction state rule: tick.induct)
+  case (1 state)
+  then show ?case 
+    by (simp add: invariant_tick)
+next
+  case (2 current big auxB)
+  then show ?case by(auto simp: size_listLength split: current.splits)
+next
+  case (3 current big auxB count)
+  then show ?case 
+    apply(auto split: current.splits)
+    (* TODO: *)
+    apply (metis Stack_Proof.pop Zero_not_Suc bot_nat_0.extremum_uniqueI empty first list.size(3) size_listLength take_Suc)
+    by (metis (no_types, lifting) One_nat_def Suc_diff_eq_diff_pred Zero_not_Suc bot_nat_0.extremum_uniqueI diff_is_0_eq empty length_greater_0_conv list.size(3) size_listLength size_pop)
+qed
 
 lemma pop: "\<lbrakk>\<not> isEmpty big; pop big = (x, big')\<rbrakk> \<Longrightarrow> x # toList big' = toList big"
   apply(induction big arbitrary: x rule: pop.induct)
@@ -39,57 +44,11 @@ next
   then show ?case by(auto split: current.splits)
 qed
 
-lemma helper_2: "\<lbrakk>
-  current = Current x1 (List.length x1) x3 (Stack.size x3); count < Stack.size x3;
-  \<not> Current.isEmpty (Current x1 (List.length x1) x3 (Stack.size x3));
-  Stack.toList x3 = drop (List.length auxB + count - Stack.size x3) (rev auxB) @ take count (Stack.toList big);
-  Stack.size x3 - count \<le> List.length auxB; 
-  get (Current x1 (List.length x1) x3 (Stack.size x3)) = (x, Current x1a x2a x3a x4);
-  big' = Reverse (Current x1a x2a x3a x4) big auxB count\<rbrakk>
-       \<Longrightarrow> Stack.toList x3a = drop (List.length auxB + count - x4) (rev auxB) @ drop (count - x4) (take count (Stack.toList big))"
-proof(induction "Current x1 (List.length x1) x3 (Stack.size x3)" rule: get.induct)
-  case 1
-  then show ?case 
-    apply auto
-    (* TODO *)
-    by (smt (z3) Nat.diff_diff_right Stack_Proof.pop Suc_diff_Suc Suc_diff_le diff_diff_cancel diff_is_0_eq helper_2 leD le_diff_conv length_0_conv length_drop length_rev less_imp_le not_less_eq rev_take tl_append2)
-next
-  case (2 x xs)
-  then show ?case by auto
-qed
-
-lemma helper_3: "\<lbrakk>current = Current x1 (List.length x1) x3 (Stack.size x3); count < Stack.size x3;
-        \<not> Current.isEmpty (Current x1 (List.length x1) x3 (Stack.size x3));
-        Stack.toList x3 = drop (List.length auxB + count - Stack.size x3) (rev auxB) @ take count (Stack.toList big);
-        Stack.size x3 - count \<le> List.length auxB; get (Current x1 (List.length x1) x3 (Stack.size x3)) = (x, Current x1a x2a x3a x4);
-        big' = Reverse (Current x1a x2a x3a x4) big auxB count\<rbrakk>
-       \<Longrightarrow> x4 - count \<le> List.length auxB"
-proof(induction "Current x1 (List.length x1) x3 (Stack.size x3)" rule: get.induct)
-  case 1
-then show ?case by auto
-next
-  case (2 x xs)
-  then show ?case by auto
-qed
-
-lemma helper_4: "\<lbrakk>
-  current = Current x1 (List.length x1) x3 (Stack.size x3);
-  count < Stack.size x3;
-  \<not> Current.isEmpty (Current x1 (List.length x1) x3 (Stack.size x3));
-  Stack.toList x3 = drop (List.length auxB + count - Stack.size x3) (rev auxB) @ take count (Stack.toList big);
-  Stack.size x3 - count \<le> List.length auxB; get (Current x1 (List.length x1) x3 (Stack.size x3)) = (x, Current x1a x2a x3a x4);
-  big' = Reverse (Current x1a x2a x3a x4) big auxB count
-\<rbrakk> \<Longrightarrow> count \<le> x4"
-proof(induction "Current x1 (List.length x1) x3 (Stack.size x3)" rule: get.induct)
-case 1
-  then show ?case by auto
-next
-  case (2 x xs)
-  then show ?case by auto
-qed
-
-lemma invariant_pop: "\<lbrakk>\<not> isEmpty big; invariant big; pop_invariant big; pop big = (x, big')\<rbrakk>
-   \<Longrightarrow> invariant big'"
+lemma invariant_pop: "\<lbrakk>
+  \<not> isEmpty big; invariant big;
+  pop_invariant big;
+  pop big = (x, big')
+\<rbrakk> \<Longrightarrow> invariant big'"
 proof(induction big arbitrary: x rule: pop.induct)
   case (1 state)
   then show ?case
@@ -97,12 +56,17 @@ proof(induction big arbitrary: x rule: pop.induct)
 next
   case (2 current big auxB count)
   then show ?case
-    apply(auto split: current.splits prod.splits)
-  (* TODO: *)
-    apply (meson Big_Proof.helper_2)
-       apply (meson Current.invariant.simps invariant_get)+
-     apply (meson helper_3)
-    by (meson helper_4)
+  proof(induction current rule: get.induct)
+    case (1 added old remained)
+    then show ?case 
+      apply auto 
+      (* TODO: *)
+      apply (smt (verit, best) Cons_nth_drop_Suc Stack_Proof.pop Suc_diff_le diff_diff_cancel diff_is_0_eq drop_all_iff le_diff_conv le_eq_less_or_eq length_rev list.sel(3) nat_neq_iff ordered_cancel_comm_monoid_diff_class.diff_diff_right tl_append2)
+      by linarith+
+  next
+    case (2 x xs added old remained)
+    then show ?case by auto
+  qed
 qed
 
 end
