Idle_Proof.thy
@@ -10,6 +10,22 @@ lemma size_push: "size (push x idle) = Suc (size idle)"
   apply(induction idle arbitrary: x)
   by(auto simp: Stack_Proof.size_push)
 
+lemma pop: "\<lbrakk>\<not> isEmpty idle; pop idle = (x, idle')\<rbrakk> \<Longrightarrow> x # toList idle' = toList idle"
+  apply(induction idle arbitrary: x)
+  by(auto simp: pop first_pop first not_empty_2)
 
+lemma size_pop: "\<lbrakk>\<not> isEmpty idle; pop idle = (x, idle')\<rbrakk> \<Longrightarrow> Suc (size idle')  = size idle"
+  apply(induction idle arbitrary: x)
+  apply(auto simp: Stack_Proof.size_pop)
+  by (simp add: not_empty_2 size_listLength)
+
+lemma invariant_push: "invariant idle \<Longrightarrow> invariant (push x idle)"
+  apply(induction x idle rule: push.induct)
+  by(auto simp: Stack_Proof.size_push)
+
+lemma invariant_pop: "\<lbrakk>\<not> isEmpty idle; invariant idle; pop idle = (x, idle')\<rbrakk>
+   \<Longrightarrow> invariant idle'"
+  apply(induction idle arbitrary: x rule: pop.induct)
+  by(auto simp: Stack_Proof.size_pop)
 
 end
